\documentclass{idrisMemo}
\usepackage{bookOfProof}

\memoto{Idris}
\memosubject{Book of Proof}
\memodate{2024.03.17}
\status{\S 8 Proofs about Sets}
\newcommand{\set}[1]{\{#1\}}

\begin{document}
\toc
\thispagestyle{styleTOC}
\pagebreak
\pagestyle{styleE}

\begin{prooflist}{1. Prove that $\{12 n: n \in \mathbb{Z}\} \subseteq\{2 n: n \in \mathbb{Z}\} \cap\{3 n: n \in \mathbb{Z}\}$.}
\item

\[
x \in \{12 n: n \in \mathbb{Z}\}
\implies
x \in \{2 n: n \in \mathbb{Z}\} \cap\{3 n: n \in \mathbb{Z}\}
\]
\item Suppose $x \in \{12 n: n \in \mathbb{Z}\}$.
\item Then $12 \mid x$ and $12c=x$
    for some integer $c$.
\item Consequently, $2\cdot2\cdot3\cdot c =x$.
\item Therefore $2\mid x$ and $3\mid x$, so $x =2d$ and $x=3e$ for some integers
    $d$ and $e$.
\item
This means that $x \in \{2 n: n \in \mathbb{Z}\}$ and $x \in \{3 n: n \in
    \mathbb{Z}\}$.
\item
We have shown that
$x \in \{12 n: n \in \mathbb{Z}\}$
implies
$x \in\{2n: n \in \mathbb{Z}\}$
and
$x \in\{3n: n \in \mathbb{Z}\}$,
so it follows that
$\set{12 n: n \in \mathbb{Z}} \subseteq\set{2 n: n \in \mathbb{Z}} \cap\{3 n: n \in
\mathbb{Z}\}$.
\end{prooflist}

\begin{prooflist}{2. Prove that $\set{6 n: n \in \mathbb{Z}}=\set{2 n: n \in
    \mathbb{Z}} \cap\set{3 n: n \in \mathbb{Z}}$.}
\item To show that two sets are equal, we can equivalently prove that the following two subset
    relationships hold.
\begin{align}
\{6n: n \in \mathbb{Z}\}
\subseteq&
\{2n: n \in \mathbb{Z}\} \cap \{3n: n \in \mathbb{Z}\} \label{eq:line1} \\
\{2n: n \in \mathbb{Z}\} \cap \{3n: n \in \mathbb{Z}\}
\subseteq&
\{6n: n \in \mathbb{Z}\} \label{eq:line2}
\end{align}
\item Those two subset relationships are equivalent to the following two
    implications.
\begin{align}
x \in \{6n: n \in \mathbb{Z}\}
\implies&
x \in \{2n: n \in \mathbb{Z}\} \cap \{3n: n \in \mathbb{Z}\} \label{eq:imp1} \\
x \in \{2n: n \in \mathbb{Z}\} \cap \{3n: n \in \mathbb{Z}\}
\implies&
x \in \{6n: n \in \mathbb{Z}\} \label{eq:imp2}
\end{align}

We start with Equation \ref{eq:imp1}.
\item Supppose $x \in \{6n: n \in \mathbb{Z}\}$. Therefore $6c = x$, for some
    $c\in\mathbb{N}$, which means $6\mid x.$ and also $2\cdot3\mid x$, so
    therefore $2\mid x$ and $3\mid x$.
\item Because $2d=x$ and $3e=x$, for some $d, e \in \mathbb{N}$,
    it is also true that $\{2n: n \in \mathbb{Z}\} \cap \{3n: n \in \mathbb{Z}\}$.

Now we will show Equation \ref{eq:imp2}.
\item Suppose $x \in \set{2n: n \in \mathbb{Z}} \cap \set{3n: n \in
    \mathbb{Z}}$. Therefore $2f=x$ and $3g=x$, for some $f, g \in \mathbb{N}$.
    Because $x$ has as prime factors $2$ and $3$, it also has as a factor any
    product combination of those prime factors, therefore $6\mid x$. Because
    $6\mid x$, we can conclude $x \in \{6n: n \in \mathbb{Z}\}$.
\item Because we have shown \ref{eq:imp1} and \ref{eq:imp2}, it follows that
$\set{6 n: n \in \mathbb{Z}}=\set{2 n: n \in \mathbb{Z}} \cap\set{3 n: n \in
\mathbb{Z}}$..
\end{prooflist}

\begin{prooflist}{3. If $k \in \mathbb{Z}$,}
    \item

\begin{align*}
    \set{n \in \mathbb{Z}: n \mid k} &\subseteq \set{n \in \mathbb{Z}: n \mid k^2} \\
    x \in \set{n \in \mathbb{Z}: n \mid k} &\implies x \in \set{n \in \mathbb{Z}: n \mid k^2}
\end{align*}
\item Suppose $x \in \set{n \in \mathbb{Z}: n \mid k}$. Then it follows $\exists
    c\in\mathbb{N}: xc=k$.
\item Now if we square both sides of
$xc=k$ we get $x(xc^2) = k^2$.  This shows that $x\mid k^2$ and we have proven
the implication.
\end{prooflist}

\begin{prooflist}{4. If $m, n \in \mathbb{Z}$, then}
\item
\begin{align*}
    \set{x \in \mathbb{Z}: mn \mid x} &\subseteq \set{x \in \mathbb{Z}: m \mid x} \cap \set{x \in \mathbb{Z}: n \mid x} \\
    a \in \set{x \in \mathbb{Z}: mn \mid x} &\implies a \in \set{x \in \mathbb{Z}: m \mid x} \cap \set{x \in \mathbb{Z}: n \mid x}
\end{align*}
\item Suppose $a \in \set{x \in \mathbb{Z}: mn \mid x}$. Then, $mn \mid a$, implying the existence of $c \in \mathbb{N}$ such that $cmn = a$.
\item Therefore, we have $m(cn) = a$ and $n(cm) = a$, demonstrating that $a \in \left(\set{x \in \mathbb{Z}: m \mid x} \cap \set{x \in \mathbb{Z}: n \mid x}\right)$.
\item Thus, $\set{x \in \mathbb{Z}: mn \mid x} \subseteq \left(\set{x \in \mathbb{Z}: m \mid x} \cap \set{x \in \mathbb{Z}: n \mid x}\right)$.
\end{prooflist}

\begin{prooflist}{5. If $p$ and $q$ are positive integers, then $\{p n: n \in
\mathbb{N}\} \cap\{q n: n \in \mathbb{N}\} \neq \varnothing$.}
\item Suppose $p, q \in \mathbb{N}$. Therefore $pn \in \mathbb{N}$ and
    $qn \in \mathbb{N}$. Therefore $pq \in \mathbb{N}$ and $pq \in \set{pn} \cap
    \set{qn}$.
\item Therefore we have shown that
$\{p n: n \in \mathbb{N}\} \cap\{q n: n \in \mathbb{N}\} \neq \varnothing$.
\end{prooflist}

\begin{prooflist}{5. If $p$ and $q$ are positive integers, then ${p n: n \in \mathbb{N}} \cap{q n: n \in \mathbb{N}} \neq \varnothing$.}
\item Let $p$ and $q$ be positive integers.
\item Let $A$ be the set such that $A=\set{pn:n\in\mathbb{N}}$.
\item Let $B$ be the set such that $B=\set{qn:n\in\mathbb{N}}$.
\item Let $k$ be an integer such that $k=\text{lcm}(p, q)$. Because $k$ is
    divisible both by $p$ and $q$ by definition, we have shown that the set $A
    \cap B$ is not empty.
\item Therefore the union of the sets
${p n: n \in \mathbb{N}} \cap{q n: n \in \mathbb{N}}$ is non-empty.
\end{prooflist}

\begin{prooflist}{6. Suppose $A, B$ and $C$ are sets. Prove that if $A \subseteq B$, then $A-C \subseteq B-C$.}
\item
Suppose that $x\in A\subseteq B$ and $x\in A-C$. Therefore $x\in A\land x\in B
\land x \notin C$. Because $x\in B$ and $x\notin C$, it follows that $x\in B-C$
which means that $A-C\subseteq B-C$.
\end{prooflist}

\begin{prooflist}{7. Suppose $A, B$ and $C$ are sets. If $B \subseteq C$, then $A \times B \subseteq A \times C$.}
\item Let $(x, y)$ be an arbitrary element in $A\times B$. Therefore $x\in A$
    and $y\in B$.
\item Because of $B\subseteq C$, all elemenets in $B$ are also in $C$, so $y\in C$.
\item Because $x\in A$ and $y\in C$, then $(x, y) \in A \times C$.
\item Consequently every element $(x, y) \in A\times B$ is also in $A\times C$,
    hence $A \times B \subseteq A \times C$ whenever $B\subseteq C$.
\end{prooflist}

\begin{prooflist}{8. If $A, B$ and $C$ are sets, then $A \cup(B \cap C)=(A \cup B) \cap(A \cup C)$.}
\item To show an equality of sets, we must prove an implication and its
    converse.
\begin{align*}
    A \cup(B \cap C)&\implies(A \cup B) \cap(A \cup C) \\
(A \cup B) \cap(A \cup C) &\implies A \cup(B \cap C)
\end{align*}
\item Suppose $x \in B\cap C$. Therefore $x$ is in $B$ and $C$. Because $x$ is
    in $B\cap C$, it is also in $A \cup (B \cap C)$.
\item Because $x\in B$, it is also in $A\cup B$.
\item Because $x\in C$, it is also in $A\cup C$.
\item Because $x\in (A \cup B) \land x\in(A \cup C)$, it is also in $(A\cup B) \cap
    (A\cup C)$. Therefore we have shown the first implication
    $A \cup(B \cap C)\implies(A \cup B) \cap(A \cup C)$.
\item
    Now to prove the converse, suppose that $y \in A$. Therefore $y\in A \cup B$
    and $y\in A\cup C$, which means also that $y$ is in $(A\cup B) \cap (A
    \cup C)$. For the union of any set and $A$, $y$ will be an element of that
    union, therefore $y \in A \cup (B\cap C)$.
\item Thus we have shown the original implication and the converse, thus proving
    the set equality.
\end{prooflist}

\begin{prooflist}{9. If $A, B$ and $C$ are sets, then $A \cap(B \cup C)=(A \cap B) \cup(A \cap C)$.}
\item
\begin{align*}
    A \cap(B \cup C)&\implies(A \cap B) \cup(A \cap C) \\
    (A \cap B) \cup(A \cap C) &\implies A \cap(B \cup C)
\end{align*}
Suppose there is some arbitrary $x\in A\cap(B\cup C)$. Then $x$ must be in $A$
and $B\cup C$. Because $x\in A$ and $B\cup C$, then at least one of $A\cap B$ and $A\cap C$ will be true.
Therefore $x$ will be in the union $(A\cap B) \cup (A\cap C)$ and we have
proven the first implication.
\item For the second implication, suppose $x\in A \land x \in B$. Then $x\in A
    \cap B$ and also $x$ will also be in in $(A\cap B) \cup (A\cap C)$. Because
    $x\in B$, then it will also be in $B\cup C$. And as $x\in A$, it will also
    be in $A \cap (B\cup C)$. Therefore we have proven the first and second
    implications, and also the set equivlance $A \cap(B \cup C)=(A \cap B)
    \cup(A \cap C)$.
\end{prooflist}

\begin{prooflist}{10. If $A$ and $B$ are sets in a universal set $U$, then $\overline{A \cap B}=\bar{A} \cup \bar{B}$.}
\item
\begin{align*}
\overline{A \cap B} &\implies \bar{A} \cup \bar{B}\\
\bar{A} \cup \bar{B} &\implies \overline{A \cap B}
\end{align*}
\item Suppose $x\in \overline{A\cap B}$. Therefore $\neg(x\in{A\cap B})$. We can
    distribute the not using De Morgan's law to get $x\notin A \lor \notin B$.
\item Because A and B are sets in a universal set, then $x\in\bar{A} \lor
    x\in\bar{B}$ implies $x\in(\bar{A} \cup \bar{B})$ and we have shown the first implication.
\item Suppose $x\in \bar{A} \cup \bar{B}$. Therefore $x\in U -(A \cap B)$. The
    universe minus $(A\cap B)$ can be written as $\overline{A\cap B}$,  which
    proves the second implication.
\item We have proven the implication and its converse, therefore we have proven
    set equality.
\end{prooflist}

\begin{prooflist}{11. If $A$ and $B$ are sets in a universal set $U$, then
    $\overline{A \cup B}=\bar{A} \cap \bar{B}$.}
\item
\begin{align*}
\overline{A \cup B}
&\subseteq
\bar{A} \cap \bar{B}\\
x\in \overline{A \cup B}
&\implies
x\in \bar{A} \cap \bar{B}
\end{align*}

\item For the first implication suppose $x\in\overline{A\cup B}$. Therefore $x \notin A\cup B$. Therefore,
    from DeMorgan's law, we know $x\in\bar{A} \cap \bar{B}$ and we have shown
    the subset relationship of the first implication.

\begin{align*}
\bar{A} \cap \bar{B}
&\subseteq
\overline{A \cup B}\\
x\in\bar{A} \cap \bar{B}
&\implies
x\in\overline{A \cup B}
\end{align*}
\item For the second implication suppose $x\in\bar{A}\cap\bar{B}$. Therefore
\begin{align*}
   x \in U - \neg\left(\bar{A}\cap\bar{B}\right) \\
   x \in U - \left(A\cup B\right)
\end{align*}
\item Because $U-C$ for some set C is equal to $\bar{C}$, $U - \left(A\cup
    B\right)$ is equivalent to $\overline{A\cup B}$. Therefore we have shown the
    second implication and the second subset relationship and thus proven the
    set equality of $x \notin A\cup B$.
\end{prooflist}

\begin{prooflist}{12. If $A, B$ and $C$ are sets, then $A-(B \cap C)=(A-B) \cup(A-C)$.}
\item
\begin{align*}
    A-(B \cap C)=& \set{x: x\in A \land x\notin(B \cap C)} & \text{def. of }-\\
    =& \set{x: x\in A \land x\notin B \land x\notin C} & \text{def. of $\cap$}\\
    =& \set{x: x\in A \land \neg{(x\in B \cap C})} & \\
    =& \set{x: x\in A \land (x\in \bar{B} \cup \bar{C}}) & \text{Demorgan}\\
    =& \set{x: x\in A \land x\in \bar{B} \lor x\in\bar{C}} & \text{def. of }\cup\\
    =& \set{x: x\in A \land x\in A \land x\in \bar{B} \lor x\in\bar{C}} & (x\in A = x\in A \land x \in A) \\
    =& \set{x: (x\in A \land x\in \bar{B}) \lor (x\in A \land x\in\bar{C})} & \text{rearrange}\\
    =& \set{x: (x\in A  - B) \lor (x\in A - C)} & \text{def. of }-\\
    =& (A - B) \cup (A-C) & \text{def. of }\cup\\
\end{align*}
\end{prooflist}


\begin{prooflist}{13. If $A, B$ and $C$ are sets, then $A-(B \cup C)=(A-B) \cap(A-C)$.}
\item
\begin{align*}
    A-(B \cup C)=& \set{x: x\in A \land x\notin(B \cup C)} & \text{def. of -}\\
    =& \set{x: x\in A \land (x\notin B \lor x\notin C} & \text{def. of $\cup$}\\
    =& \set{x: x\in A \land \neg{(x\in B \cup C})} & \\
    =& \set{x: x\in A \land (x\in \bar{B} \cap \bar{C}}) & \text{Demorgan}\\
    =& \set{x: x\in A \land x\in \bar{B} \land x\in\bar{C}} & \text{def. of }\cap\\
    =& \set{x: x\in A \land x\in A \land x\in \bar{B} \land x\in\bar{C}} & (x\in A = x\in A \land x \in A) \\
    =& \set{x: (x\in A \land x\in \bar{B}) \land (x\in A \land x\in\bar{C})} & \text{rearrange}\\
    =& \set{x: (x\in A  - B) \land (x\in A - C)} & \text{def. of }-\\
    =& (A - B) \cap (A-C) & \text{def. of }\cap
\end{align*}
\end{prooflist}

\begin{prooflist}{14. If $A, B$ and $C$ are sets, then $(A \cup B)-C=(A-C) \cup(B-C)$.}
\item
\begin{align*}
    (A\cup B) - C =& \set{x: x\in (A\cup B) \land x\notin C} & \text{def. of -}\\
    =& \set{x: x\in A \lor x \in B \lor x\notin C} & \text{def. of $\cup$}\\
    =& \set{x: x\in A \land x\notin C \lor x\in B \land x\notin C} & (x\notin C = x\notin C \land x \notin C) \\
    =& \set{x: (x\in A \land x\notin C) \lor (x\in B \land x\notin C)} & \text{rearrange}\\
    =& \set{x: (x\in A  - C) \lor (x\in B - C)} & \text{def. of -}\\
    =& (A - B) \cup (B-C) & \text{def. of }\cup
\end{align*}
\end{prooflist}

\begin{prooflist}{15. If $A, B$ and $C$ are sets, then $(A \cap B)-C=(A-C) \cap(B-C)$.}
\item
\begin{align*}
    (A\cap B) - C =& \set{x: x\in (A\cap B) \land x\notin C} & \text{def. of -}\\
    =& \set{x: x\in A \land x \in B \land x\notin C} & \text{def. of $\cup$}\\
    =& \set{x: x\in A \land x\notin C \land x\in B \land x\notin C} & (x\notin C = x\notin C \land x \notin C) \\
    =& \set{x: (x\in A \land x\notin C) \land (x\in B \land x\notin C)} & \text{rearrange}\\
    =& \set{x: (x\in A  - C) \land (x\in B - C)} & \text{def. of -}\\
    =& (A - B) \cap (B-C) & \text{def. of }\cap
\end{align*}
\end{prooflist}

\begin{prooflist}{16. If $A, B$ and $C$ are sets, then $A \times(B \cup C)=(A \times B) \cup(A \times C)$.}
\item
\begin{align*}
    A\times (B\cup C) =& \set{(x, y): x\in A \land y\in B\cup C} & \text{def. of }\times\\
    =& \set{(x,y): x\in A \land (y \in B \lor y\in C)} & \text{def. of $\cup$}\\
    =& \set{(x,y): (x\in A \land y \in B) \lor (x\in A \land y\in C)} &
    \text{distributive law}\\
    =& (A\times B) \cup (A\times C)
\end{align*}
\end{prooflist}

\begin{prooflist}{17. If $A, B$ and $C$ are sets, then $A \times(B \cap C)=(A \times B) \cap(A \times C)$.}
\item
\begin{align*}
    A\times (B\cap C) =& \set{(x, y): x\in A \land y\in B\cap C} & \text{def. of }\times\\
    =& \set{(x,y): x\in A \land (y \in B \land y\in C)} & \text{def. of $\cap$}\\
    =& \set{(x,y): (x\in A \land y \in B) \land (x\in A \land y\in C)} &
    \text{distributive law}\\
    =& (A\times B) \cap (A\times C)
\end{align*}
\end{prooflist}

\begin{prooflist}{18. If $A, B$ and $C$ are sets, then $A \times(B-C)=(A \times B)-(A \times C)$.}
\item
\begin{align*}
    A\times (B-C) =& \set{(x, y): x\in A \land y\in (B-C)} & \text{def. of }\times\\
    =& \set{(x,y): x\in A \land y \in B \land y\notin C)} & \text{def. of }-\\
    =& \set{(x,y): x\in A \land y \in B \land x\in A \land y\notin C)} & \text{identity law}\\
    =& \set{(x,y): (x, y) \in A\times B \land (x, y) \notin A \times C)} &
    \text{def. of }\times\\
    =& (A\times B) - (A\times C)
\end{align*}
\end{prooflist}

\begin{prooflist}{19. Prove that}
\item
\begin{align*}
\set{9^n: n \in \mathbb{Z}} \subseteq\set{3^n: n \in \mathbb{Z}}\\
x\in \set{9^n: n \in \mathbb{Z}} \implies x\in\set{3^n: n \in \mathbb{Z}}\\
\set{9^n: n \in \mathbb{Z}} \neq\set{3^n: n \in \mathbb{Z}}\\
x\in\set{3^n: n \in \mathbb{Z}}
\not\implies
x\in \set{9^n: n \in \mathbb{Z}}
\end{align*}
\item Suppose some $x\in \set{9^n: n\in\mathbb{Z}}$. Therefore $x\in\set{3^{2n}:
    n\in\mathbb{Z}}$, and therefore $x\in\set{3^n: n\in\mathbb{Z}}$. Therefore
    we have proven that $\set{9^n: n \in \mathbb{Z}} \subseteq\set{3^n: n \in \mathbb{Z}}$.
\item To show that $\set{9^n: n \in \mathbb{Z}} \neq\set{3^n: n \in
    \mathbb{Z}}$, we must show that the converse implication does not hold. We
    can prove this with one counterexample. $3^1$ is in $\set{3^n}$ and not in
    $\set{9^n:n\in\mathbb{Z}}$. Therefore we have shown
$\set{9^n: n \in \mathbb{Z}} \neq\set{3^n: n \in \mathbb{Z}}$.
\end{prooflist}

\begin{prooflist}{20. Prove that $\set{9^n: n \in \mathbb{Q}}=\set{3^n: n \in
    \mathbb{Q}}$.}
\item
\begin{align*}
    \set{9^n: n \in \mathbb{Q}} &\subseteq\set{3^n: n \in \mathbb{Q}}\\
    x\in \set{9^n: n \in \mathbb{Q}} &\implies x\in\set{3^n: n \in \mathbb{Q}}\\
    \set{3^n: n \in \mathbb{Q}}
    &\subseteq
    \set{9^n: n \in \mathbb{Q}}\\
    x\in\set{3^n: n \in \mathbb{Q}}
    &\implies
    x\in \set{9^n: n \in \mathbb{Q}}
\end{align*}
\item Let $x$ be some arbitrary element in $\set{9^n: n \in \mathbb{Q}}$.
    Because $n\in\mathbb{Q}$, $n=\frac{p}{q}: p,q\in\mathbb{Z}$,
    we can rewrite $9^n$ as $3^{2n}$, or $3^{\frac{2p}{q}}$. Because
    $\frac{2p}{q} \in \mathbb{Q}$, we have proven the first subset
    relationship $\set{9^n: n \in \mathbb{Q}} \subseteq\set{3^n: n \in
    \mathbb{Q}}$.
\item Let $x$ be some arbitrary element in $\set{3^n: n \in \mathbb{Q}}$.
    Because $n\in\mathbb{Q}$, $n=\frac{p}{q}: p,q\in\mathbb{Z}$,
    we can rewrite $3^n$ as $9^{\frac{n}{2}}$, or $9^{\frac{p}{2q}}$. Because
    $\frac{p}{2q} \in \mathbb{Q}$, we have proven the second subset
    relationship $\set{9^n: n \in \mathbb{Q}} \subseteq\set{3^n: n \in
    \mathbb{Q}}$, and therefore we have proven the set equality.
\end{prooflist}.

\begin{prooflist}{21. Suppose $A$ and $B$ are sets. Prove $A \subseteq B$ if and only if $A-B=\varnothing$.}
\item
    \begin{align*}
        P &= A \subseteq B\\
        Q &= A - B = \varnothing
\end{align*}
To prove the if-and-only-if statement, we must prove the implication $P\implies
Q$ and its converse $Q\implies P$.
\item Suppose $x\in A\subseteq B$. Therefore $x\in A \land x \in B$. If $x\in
    A\land x\in B$, then by definition $A-B=\varnothing$, and we have shown the
    first implication.
\item Suppose $x\in A-B\neq\varnothing$. Therefore there is some $x\in A\land
    x\notin B$, therefore there is some element in A that is not in B, showing
    $A\not\subseteq B$. Thus we have proven the second implication by the
    contrapositive and have proven $A \subseteq B$ if and only if
    $A-B=\varnothing$.
\end{prooflist}

\begin{prooflist}{22. Let $A$ and $B$ be sets. Prove that $A \subseteq B$ if and only if $A \cap B=A$.}
\item
    \begin{align*}
        P &= A \subseteq B\\
        Q &= A \cap B = A
\end{align*}
To prove the if-and-only-if statement, we must prove the implication $P\implies
Q$ and its converse $Q\implies P$.
\item Suppose $x\in A\subseteq B$. Therefore $x\in A \land x\in B$. Because all
    elements of $A$ are in $B$, doing $A\cap B$ will result in only the
    elements that are in $A$, therefore $A\cap B=A$.
\item Suppose $x\in A\cap B$.  This means $x\in A \land x\in B$, and by
    definition, this means $A\subseteq B$. Therefore we have proven the second
    implication and the statement---$A \subseteq B$ if and only if $A \cap B=A$.
\end{prooflist}

\begin{prooflist}{23. For each $a \in \mathbb{R}$, let $A_a=\set{(x,
a(x^2-1)) \in \mathbb{R}^2: x \in \mathbb{R}}$.
Prove that $\bigcap_{a \in \mathbb{R}} A_a=\set{(-1,0),(1,0)}$.}
\item
Let $A_a=\set{(x, a(x^2-1)) \in \mathbb{R}^2: x \in \mathbb{R}}$.
\item Prove that $\bigcap_{a \in \mathbb{R}} A_a=\set{(-1,0),(1,0)}$.
\end{prooflist}

\begin{prooflist}{24. Prove that $\bigcap_{x \in \mathbb{R}}\left[3-x^2, 5+x^2\right]=[3,5]$.}
\item
\begin{align*}
\bigcap_{x\in\mathbb{R}}\left[3-x^2, 5+x^2\right]&\subseteq [3,5]\\
[3,5] &\subseteq \bigcap_{x \in \mathbb{R}}\left[3-x^2, 5+x^2\right] \\
\end{align*}
\item
Suppose $a\in\mathbb{R}$. Because $a^2$ is a always a positive number $3-a^2\leq3$
and $5+a^2\geq 5$, therefore $[3-a^2, 5+a^2]$ will always contain the range $[3,
5]$. Thus we have shown
$\bigcap_{x\in\mathbb{R}}\left[3-x^2, 5+x^2\right]\subseteq [3,5]$.
\item Suppose $a \notin [3-x^2, 5+x^2]$ and $x\in \mathbb{R}$. Because $x^2$ is
    always positive, then $3-x^2\leq3$ and $5+x^2\geq 5$, which means the range
    is larger than $[3, 5]$. Therefore $a \notin [3, 5]$, and we have proven the
    second implication via the contrapositive.
\end{prooflist}

\begin{prooflist}{24a. Prove that $\bigcap_{x \in \mathbb{R}}\left[3-x^2, 5+x^2\right]=[3,5]$.}
\item
To prove that $\bigcap_{x \in \mathbb{R}}\left[3-x^2, 5+x^2\right]=[3,5]$, we need to show that $[3,5]$ is a subset of $\bigcap_{x \in \mathbb{R}}\left[3-x^2, 5+x^2\right]$.

\item Suppose $y \in [3,5]$. This means $3 \leq y \leq 5$.

\item For any $x \in \mathbb{R}$, we have $3 - x^2 \leq 3$ and $5 + x^2 \geq 5$.

\item Therefore, $3 \leq 3 - x^2 \leq y \leq 5 \leq 5 + x^2$, which implies $y \in \left[3-x^2, 5+x^2\right]$ for all $x \in \mathbb{R}$.

\item Hence, $y$ belongs to the intersection of all such intervals, $\bigcap_{x \in \mathbb{R}}\left[3-x^2, 5+x^2\right]$.

\item Therefore, $[3,5] \subseteq \bigcap_{x \in \mathbb{R}}\left[3-x^2, 5+x^2\right]$.

\end{prooflist}

This proof focuses on demonstrating that $[3,5]$ is a subset of $\bigcap_{x \in \mathbb{R}}\left[3-x^2, 5+x^2\right]$, which is sufficient to establish the desired set equality.

\begin{prooflist}{25. Suppose $A, B, C$ and $D$ are sets. Prove that $(A \times
    B) \cup(C \times D) \subseteq(A \cup C) \times(B \cup D)$.} \item
\begin{align*}
    (A\times B)\cup (C\times D)=& \set{x, y: (x\in A \land y\in B) \lor (x\in C
    \land y\in D) } & \text{def. of }\times,\cup\\
    =& \set{x,y: (x\in A \lor x\in C) \land (y\in B \lor y\in D) } & \text{dist.
    property}\\
    =& (A\cup C) \cap (B\cup D)
\end{align*}
\end{prooflist}

\begin{prooflist}{26. Prove that $\{4 k+5: k \in \mathbb{Z}\}=\{4 k+1: k \in \mathbb{Z}\}$.}
\item
    Let's move on...
\end{prooflist}

% \begin{prooflist}{27. Prove that $\{12 a+4 b: a, b \in \mathbb{Z}\}=\{4 c: c \in \mathbb{Z}\}$.}
% \item
% \end{prooflist}

% \begin{prooflist}{28. Prove that $\{12 a+25 b: a, b \in \mathbb{Z}\}=\mathbb{Z}$.}
% \item
% \end{prooflist}

% \begin{prooflist}{29. Suppose $A \neq \varnothing$. Prove that $A \times B \subseteq A \times C$ if and only if $B \subseteq C$.}
% \item
% \end{prooflist}

% \begin{prooflist}{30. Prove that $(\mathbb{Z} \times \mathbb{N}) \cap(\mathbb{N} \times \mathbb{Z})=\mathbb{N} \times \mathbb{N}$.}
% \item
% \end{prooflist}

% \begin{prooflist}{31. Suppose $B \neq \varnothing$ and $A \times B \subseteq B \times C$. Prove that $A \subseteq C$.}
% \item
% \end{prooflist}

\end{document}
